- uniqueness - some useful properties - setSize union-rule

inc/SetPcpo.thy
@@ -197,14 +197,14 @@ lemma union_cont:"cont (\<lambda>S2. union S1 S2)"
   by (metis (no_types, lifting) UN_simps(3) Union_is_lub empty_not_UNIV lub_eq lub_eqI)
 
 
-inductive setSize_helper :: "'a set \<Rightarrow> lnat \<Rightarrow> bool"
+inductive setSize_helper :: "'a set \<Rightarrow> nat \<Rightarrow> bool"
   where
-    "setSize_helper {} (Fin 0)"
-  |  "setSize_helper A (Fin X) \<and> a \<notin> A \<Longrightarrow> setSize_helper (insert a A) (Fin (Suc X))"
+    "setSize_helper {} 0"
+  |  "setSize_helper A X \<and> a \<notin> A \<Longrightarrow> setSize_helper (insert a A) (Suc X)"
 
 definition setSize :: "'a set \<Rightarrow> lnat"
   where
-  "setSize X \<equiv> if (finite X) then (SOME Y. setSize_helper X Y) else \<infinity>"
+  "setSize X \<equiv> if (finite X) then Fin (THE Y. setSize_helper X Y) else \<infinity>"
 
 
 lemma setSizeEx: assumes "finite X" shows "\<exists> Y. setSize_helper X Y"
@@ -213,21 +213,103 @@ lemma setSizeEx: assumes "finite X" shows "\<exists> Y. setSize_helper X Y"
   using setSize_helper.intros(1) apply auto[1]
   by (metis setSize_helper.simps)
 
-(* (*would be nice to prove this lemmas*)
-lemma setSizeBack: assumes "finite F" 
-  shows "setSize_helper (insert x F) (Fin (Suc A)) \<and> x \<notin> F \<longrightarrow> setSize_helper F (Fin A)"
-  apply (rule finite_induct)
-  apply (simp add: assms)
-  apply (metis Suc_inject inject_Fin insert_eq_iff insert_not_empty setSize_helper.simps)
-  oops
+lemma setSize_remove: "y \<in> F \<and> setSize_helper (F - {y}) A \<longrightarrow> setSize_helper F (Suc A)"
+  by (metis Diff_insert_absorb Set.set_insert setSize_helper.intros(2))
 
-lemma setSizeonlyOne: 
-  assumes "finite X" 
-  shows "\<forall>Y. \<forall>Z. setSize_helper X Y \<and> Z \<noteq> Y \<longrightarrow> \<not> (setSize_helper X Z)"
+
+lemma setSizeBack_helper:  
+  assumes "\<forall>(F::'a set) x::'a. (finite F \<and> setSize_helper (insert x F) (Suc A) \<and> x \<notin> F) \<longrightarrow> setSize_helper F A"
+  shows "\<forall>(F::'a set) x::'a. (finite F \<and> setSize_helper (insert x F) (Suc (Suc A)) \<and> x \<notin> F) \<longrightarrow> setSize_helper F (Suc A)"
+proof -
+have b0: "\<And>A::nat. \<forall>(F::'a set) x::'a. ((setSize_helper (insert x F) (Suc (Suc A)) \<and> x \<notin> F) 
+  \<longrightarrow> (\<exists> y. y \<in> (insert x F) \<and> setSize_helper ((insert x F) - {y}) (Suc A)))"
+    by (metis Diff_insert_absorb add_diff_cancel_left' insertI1 insert_not_empty plus_1_eq_Suc setSize_helper.simps)
+have b1: "\<forall>(F::'a set) (x::'a) y::'a. ((finite F \<and> setSize_helper (insert x (F - {y})) (Suc A) \<and> x \<notin> F)
+  \<longrightarrow> setSize_helper (F - {y}) A)"
+  using assms by auto
+have b2: "\<forall>(F::'a set) x::'a. (setSize_helper (insert x F) (Suc (Suc A)) \<and> x \<notin> F) 
+  \<longrightarrow> ((\<exists> y. (y\<noteq>x \<and> y \<in> F \<and> setSize_helper (insert x (F - {y})) (Suc A))) \<or> setSize_helper F (Suc A))"
+  by (metis Diff_insert_absorb b0 empty_iff insert_Diff_if insert_iff)
+have b3: "\<forall>(F::'a set) x::'a. (setSize_helper (insert x F) (Suc (Suc A)) \<and> x \<notin> F \<and> finite F) 
+  \<longrightarrow> ((\<exists> y. (y\<noteq>x \<and> y \<in> F \<and> setSize_helper (F - {y}) A)) \<or> setSize_helper F (Suc A))"
+  by (meson b1 b2)
+show "\<forall>(F::'a set) x::'a. (finite F \<and> setSize_helper (insert x F) (Suc (Suc A)) \<and> x \<notin> F) \<longrightarrow> setSize_helper F (Suc A)"
+  by (meson b3 setSize_remove)
+qed
+
+
+lemma setSizeBack: "\<And> F x. (finite F \<and> setSize_helper (insert x F) (Suc A) \<and> x \<notin> F) \<Longrightarrow> setSize_helper F A"
+  apply (induction A)
+  apply (metis Suc_inject empty_iff insertI1 insert_eq_iff nat.distinct(1) setSize_helper.simps)
+  using setSizeBack_helper by blast
+
+
+lemma setSizeonlyOne: assumes "finite X" shows "\<exists>! Y. setSize_helper X Y"
   apply (rule finite_induct)
   apply (simp add: assms)
-  apply (metis insert_not_empty setSize_helper.simps)
-  oops
-*)
+  apply (metis empty_not_insert setSize_helper.simps)
+  by (metis insert_not_empty setSizeBack setSize_helper.intros(2) setSize_helper.simps)
+
+
+lemma setSizeSuc: assumes "finite X" and "z \<notin> X" shows "setSize (insert z X) = lnsuc\<cdot>(setSize X)"
+  apply (simp add: setSize_def)
+  using assms setSizeonlyOne
+  by (metis (mono_tags, lifting) Diff_insert_absorb finite.insertI insertI1 setSize_remove theI_unique)
+
+lemma setsize_union_helper1: 
+  assumes "finite F"
+      and "x \<notin> F"
+      and "x \<notin> X"
+    shows "setSize (X \<union> F) + setSize (X \<inter> F) = setSize X + setSize F \<Longrightarrow>
+       setSize (X \<union> insert x F) + setSize (X \<inter> insert x F) = setSize X + setSize (insert x F)"
+proof - 
+  assume a0: "setSize (X \<union> F) + setSize (X \<inter> F) = setSize X + setSize F"
+  have b0: "X \<union> insert x F = insert x (X \<union> F)"
+    by simp
+  have b1: "setSize (X \<union> insert x F) = lnsuc\<cdot>(setSize (X \<union> F))"
+    by (metis Un_iff Un_infinite assms(1) assms(2) assms(3) b0 finite_UnI fold_inf setSizeSuc setSize_def sup_commute)
+  have b2: "setSize (X \<inter> insert x F) = setSize (X \<inter> F)"
+    by (simp add: assms(3)) 
+  show "setSize (X \<union> insert x F) + setSize (X \<inter> insert x F) = setSize X + setSize (insert x F)"
+    by (metis (no_types, lifting) a0 ab_semigroup_add_class.add_ac(1) add.commute assms(1) assms(2) 
+      b1 b2 lnat_plus_suc setSizeSuc)
+qed
+
+lemma setsize_union_helper2: 
+  assumes "finite F"
+      and "x \<notin> F"
+      and "x \<in> X"
+    shows "setSize (X \<union> F) + setSize (X \<inter> F) = setSize X + setSize F \<Longrightarrow>
+       setSize (X \<union> insert x F) + setSize (X \<inter> insert x F) = setSize X + setSize (insert x F)"
+proof -
+  assume a0: "setSize (X \<union> F) + setSize (X \<inter> F) = setSize X + setSize F"
+  have b0: "setSize (X \<union> insert x F) = setSize (X \<union> F)"
+    by (metis Un_Diff_cancel assms(3) insert_Diff1)
+  have b1: "setSize (X \<inter> insert x F) =  lnsuc\<cdot>(setSize (X \<inter> F))"
+    by (simp add: assms(1) assms(2) assms(3) setSizeSuc)
+  show "setSize (X \<union> insert x F) + setSize (X \<inter> insert x F) = setSize X + setSize (insert x F)"
+    by (metis a0 ab_semigroup_add_class.add_ac(1) assms(1) assms(2) b0 b1 lnat_plus_suc setSizeSuc)
+qed
+
+lemma setsize_union_helper3: assumes "finite X" and "finite Y"
+  shows "setSize (X \<union> Y) + setSize (X \<inter> Y) = setSize X + setSize Y"
+  apply (rule finite_induct)
+  apply (simp add: assms)
+  apply simp
+  by (meson setsize_union_helper1 setsize_union_helper2)
+
+lemma setsize_union_helper4: assumes "infinite X \<or> infinite Y"
+  shows "setSize (X \<union> Y) + setSize (X \<inter> Y) = setSize X + setSize Y"
+proof -
+  have b0: "setSize (X \<union> Y) = \<infinity>"
+    by (metis (full_types) assms infinite_Un setSize_def)
+  have b1: "setSize X = \<infinity> \<or> setSize Y = \<infinity>"
+    by (meson assms setSize_def)
+  show ?thesis
+    using b0 b1 plus_lnatInf_r by auto
+qed
+
+lemma setsize_union: "setSize (X \<union> Y) + setSize (X \<inter> Y) = setSize X + setSize Y"
+  by (meson setsize_union_helper3 setsize_union_helper4)
 
 end
